src/Verse/Types/Internal.v
@@ -176,10 +176,16 @@ demands.
 
 *)
 
+Require Verse.Nibble.
+
+(** Elements of the word type are represented as nibbles *)
+Definition wordRep : nat -> Type := fun n => Nibble.bytes (2^n).
+Definition ConstRep : typeC TypeDenote := mkTypeDenote wordRep.
+Import Verse.PrettyPrint.
+Global Instance constant_pretty n : PrettyPrint (wordRep n) := Nibble.pretty_print (2 * 2^n).
+
 Require Import Verse.Word.
 Definition stdWordDenote : nat -> Type := fun n => Word.bytes (2^n).
 
-Definition StandardSemantics : typeC TypeDenote := mkTypeDenote stdWordDenote.
 
-Import Verse.PrettyPrint.
-Global Instance word_constant_pretty n : PrettyPrint (stdWordDenote n) := word_pretty (8 * 2^n).
+Definition StandardSemantics : typeC TypeDenote := mkTypeDenote stdWordDenote.
